\documentclass{article}
\usepackage{amsmath}



\begin{document}

\begin{itemize}
    \item $d$ - distance travelled
    \item $v$ - velocity
    \item $cr$ - charge rate
    \item $t_t$ - travel time
    \item $t_c$ - charge time
    \item $t$ - total time
\end{itemize}

\begin{displaymath}
    \begin{cases}
        d = v \times t_t \\
        v = cr \times t_c \\
        t = t_t + t_c \\
        cr = 1 \\
    \end{cases}
\end{displaymath}

\begin{displaymath}
    t_t = t - t_c
\end{displaymath}

\begin{displaymath}
    d = 1 \times t_c \times (t - t_c)
\end{displaymath}

\begin{displaymath}
    d = t_c \times t - t_c^2
\end{displaymath}

\begin{displaymath}
    - t_c^2 + t_c \times t - d = 0
\end{displaymath}

This is quadratic equation with: $a = -1$, $b = t$ and $c = -d$.

Calculate discriminant:

\begin{displaymath}
    \Delta = t^2 - 4 \times (-1) \times (-d)
\end{displaymath}

\begin{displaymath}
    \Delta = t^2 - 4 \times d
\end{displaymath}


Roots:
\begin{displaymath}
    \frac{t \pm \sqrt{\Delta}}{2}\\
\end{displaymath}


The expected result is distance between roots:

\begin{displaymath}
    res = \frac{t + \sqrt{\Delta}}{2} - \frac{t - \sqrt{\Delta}}{2}
\end{displaymath}

\begin{displaymath}
    res = \frac{t + \sqrt{\Delta} - t + \sqrt{\Delta}}{2}
\end{displaymath}

\begin{displaymath}
    res = \frac{\sqrt{\Delta} \times 2}{2}
\end{displaymath}





Arriving at final expression:
\begin{equation}
    res = \sqrt{t^2 - 4 \times d}
\end{equation}


\end{document}
